proof/AdequacySound.v
@@ -176,15 +176,14 @@ Section ADQSOUND.
     { eapply SkEnv.load_skenv_wf; et. }
     assert(GE: sound_ge su_init m_init).
     { econs. rewrite Forall_forall. intros ? IN. ss. des_ifs. u in IN.
-      rewrite Midx.in_mapi_iff in IN.
+      rewrite in_map_iff in IN.
       des; ss; clarify.
       + s. split; ss; try apply Sound.system_skenv; eauto.
-      + assert(INCL: SkEnv.includes (Sk.load_skenv sk_link_src) (Mod.sk a)).
-        { unfold p_src in IN0. unfold ProgPair.src in *. apply nth_error_map_some in IN0.
-          des. des_ifs. eapply INCLSRC; et. eapply nth_error_In; eauto. }
+      + assert(INCL: SkEnv.includes (Sk.load_skenv sk_link_src) (Mod.sk x0)).
+        { unfold p_src in IN0. unfold ProgPair.src in *. rewrite in_map_iff in IN0. des. clarify. eapply INCLSRC; et. }
         split; ss.
         * eapply Sound.skenv_project; eauto.
-          { eapply link_load_skenv_wf_mem; et. eapply nth_error_In; eauto. }
+          { eapply link_load_skenv_wf_mem; et. }
           rewrite <- Mod.get_modsem_skenv_spec; ss. eapply SkEnv.project_impl_spec; et.
         * rewrite Mod.get_modsem_skenv_link_spec. ss.
     }
@@ -226,12 +225,10 @@ Section ADQSOUND.
       + inv MSFIND. ss. rr in SIMPROG. rewrite Forall_forall in *. des; clarify.
         { eapply system_local_preservation. }
         u in MODSEM.
-        rewrite Midx.in_mapi_iff in MODSEM.
-        des; clarify. rename a into md_src.
+        rewrite in_map_iff in MODSEM.
+        des; clarify. rename x into md_src.
         assert(exists mp, In mp pp /\ mp.(ModPair.src) = md_src).
-        { clear - MODSEM0. rr in pp. rr in p_src. subst p_src.
-          apply nth_error_map_some in MODSEM0. des.
-          esplits; eauto. { eapply nth_error_In; eauto. } }
+        { clear - MODSEM0. rr in pp. rr in p_src. subst p_src. rewrite in_map_iff in *. des. eauto. }
         des. exploit SIMPROG; eauto. intros MPSIM. inv MPSIM.
         destruct SIMSKENV. exploit SIMMS.
         { eapply INCLSRC; et. }
